injp_self & wt_c whihe changed valid_query

demo/DemoBproof.v
@@ -16,53 +16,111 @@ Require Import CKLRAlgebra Inject InjectFootprint.
 
 Section SELF_INJP.
 
+Section ms.
+Variable w : world injp.
+
+Inductive match_states' : state -> state -> Prop :=
+  |match_callstate_intro f m1 m2 Hm i:
+     injp_acc w (injpw f m1 m2 Hm) ->
+     match_states' (Callstate i m1) (Callstate i m2)
+  |match_Interstate_intro f m1 m2 Hm i:
+     injp_acc w (injpw f m1 m2 Hm) ->
+     match_states' (Interstate i m1) (Interstate i m2)
+  |match_Returnstate_intro f m1 m2 Hm i:
+     injp_acc w (injpw f m1 m2 Hm) ->
+     match_states' (Returnstate i m1) (Returnstate i m2).
+End ms.
+
 Theorem self_simulation_C :
   forward_simulation (cc_c injp) (cc_c injp) Bspec Bspec.
 Proof.
   constructor. econstructor; eauto. instantiate (1 := fun _ _ _ => _). cbn beta.
   intros se1 se2 w Hse Hse1. cbn in *.
-  
-Admitted.
+  pose (ms := fun s1 s2 => match_states' w s1 s2).
+  eapply forward_simulation_step with (match_states := ms); cbn; eauto.
+  - intros. inv H0. inv H. inv H4. inv H6. inv H2. inv H4. cbn in *.
+    inv Hse. inv H7.
+    eapply Genv.find_symbol_match in H; eauto. destruct H as [tb [A B]].
+    exists (Callstate i m2). split.
+    econstructor; eauto. simpl in H1. rewrite H1 in A. inv A.
+    rewrite Ptrofs.add_zero. reflexivity.
+    econstructor; eauto. reflexivity.
+  - intros. inv H; inv H0.
+    exists (cr (Vint i) m2). split; econstructor; eauto.
+    split. eauto. constructor. simpl. eauto.
+    constructor.
+  - intros. inv H; inv H0. inversion Hse. subst. eapply Genv.find_symbol_match in H as H'; eauto.
+    destruct H' as [tb [A B]]. inv H1.
+    exists (injpw f m1 m2 Hm),(cq (Vptr tb Ptrofs.zero) int_int_sg (Vint (Int.sub i (Int.repr 1)) :: nil) m2).
+    apply Mem.unchanged_on_support in H11 as SUP1.
+    apply Mem.unchanged_on_support in H12 as SUP2.
+    repeat apply conj; eauto.
+    + constructor. eauto.
+    + constructor. simpl.
+    replace (Vptr tb Ptrofs.zero) with (Vptr tb (Ptrofs.add Ptrofs.zero (Ptrofs.repr 0))).
+    econstructor; eauto. rewrite Ptrofs.add_zero. reflexivity.
+    simpl. constructor. constructor. constructor. constructor. congruence.
+    + constructor.
+      eapply Genv.match_stbls_incr; eauto.
+      intros. exploit H14; eauto. intros [C D].
+      unfold Mem.valid_block in *. split; eauto.
+      eauto. eauto.
+    + intros r1 r2 s1' [w'[ Hw Hr]] F.
+      destruct w'. inv F. inv Hr. cbn in *. inv H4.
+      inv H6.
+      exists (Returnstate (sum i) m2'). split.
+      constructor. auto.
+      econstructor; eauto.
+      etransitivity; eauto. constructor; eauto.
+  - intros. inv H0; inv H.
+    + exists (Returnstate (sum i) m2). split.
+      constructor. econstructor; eauto.
+    + exists (Interstate i m2). split.
+      constructor; auto. econstructor; eauto.
+  - constructor. intros. inv H.
+Qed.
 
 End SELF_INJP.
 
 Section WT_C.
-
+  
 Theorem self_simulation_wt :
   forward_simulation (wt_c @ lessdef_c) (wt_c @ lessdef_c) Bspec Bspec.
 Proof.
-  constructor. econstructor; eauto. instantiate (1 := fun _ _ _ => _). cbn beta.
+  constructor. econstructor; eauto.
   intros se1 se2 w Hse Hse1. cbn in *.
   destruct w as [[se1' [se2' sg]] ?]. destruct Hse as [Hse Hse2].
   subst. inv Hse.
-  eapply forward_simulation_step with (match_states:= eq).
-  - intros. inv H. inv H0. cbn in *.
-    inv H1. inv H. reflexivity.
-  - intros. inv H. inv H1. cbn in *. inv H. inv H1. exists s1.
+  instantiate (1 := fun se1 se2 w _ => (fun s1 s2 => s1 = s2 /\ snd (snd (fst w)) = int_int_sg)). cbn beta. simpl.
+  instantiate (1 := state).
+  instantiate (1 := fun s1 s2 => False).
+  constructor; eauto.
+  - intros. inv H. inv H1. cbn in *. inv H. inv H1. exists s1. exists s1.
     split. inv H2. inv H0. simpl. simpl in *.
     inv H. inv H2. inv H5.
-    econstructor; eauto. reflexivity.
-  - intros. subst.
-    inv H0. eexists.
-    split.
-    constructor.
-    eexists. split.
-    econstructor. simpl. admit. (*add WT assumptions in Bspec ?? How did they do for wt_c*)
+    econstructor; eauto. split. reflexivity.
+    inv H0. reflexivity.
+  - intros. inv H. exists r1.
+    split. auto. exists r1. inv H0.
+    split; simpl; auto.
+    econstructor; simpl. eauto.
     econstructor. constructor.
   - intros. subst.
     exists (se2 , (se2, int_int_sg), tt).
-    exists q1. repeat apply conj; simpl; auto.
+    exists q1. inv H. repeat apply conj; simpl; auto.
     + exists q1. split; inv H0; simpl;  constructor; simpl; eauto.
     + constructor; eauto. simpl. constructor. eauto.
-    + intros. exists s1'. split; eauto.
+    + intros. exists s1'. exists s1'. split; eauto.
       destruct H as [r3 [A B]].
       inv A. inv B. inv H1. inv H2. constructor. auto.
-  - intros. subst. exists s1'. eauto.
-  - constructor. intros.
-    constructor. inv H.
-Admitted.
+  - intros. inv H0. exists s1', s1'. split. left. econstructor; eauto.
+    econstructor. traceEq.
+    eauto.
+  - constructor. intros. inv H.
+Qed.
 
 End WT_C.
+
 
 Variable BspecL : Smallstep.semantics li_locset li_locset.
 Variable BspecM : Smallstep.semantics li_mach li_mach.
@@ -101,7 +159,6 @@ End Ainj.
 Theorem Bproof :
   forward_simulation cc_compcert cc_compcert Bspec (Asm.semantics DemoB.prog).
 Proof.
-  
   unfold cc_compcert.
   rewrite <- (cc_compose_assoc wt_c lessdef_c) at 1.
   rewrite <- (cc_compose_assoc wt_c lessdef_c).
